io/Hyperproperties.fst
@@ -1,0 +1,78 @@
+module Hyperproperties
+
+open FStar.Tactics
+open ExtraTactics
+open FStar.Ghost
+open FStar.String
+
+open IIO
+open BeyondCriteria
+open IIO.Behavior
+
+(** There are many difficulties on trying to state Hyperproperties
+about whole/partial source programs. **)
+
+(** Whole programs **)
+
+let read_content (fnm:string) : IIO (r:(resexn string){~(r == Inr Contract_failure)}) IOActions
+  (requires (fun _ -> True))
+  (ensures (fun _ r lt -> 
+    (Inr? r /\ lt == [EOpenfile fnm (Inr (Inr?.v r))]) \/
+    (exists fd. lt == [EOpenfile fnm (Inl fd);ERead fd r])
+    )) =
+  match static_cmd Openfile fnm with
+  | Inl fd -> static_cmd Read fd
+  | Inr err -> Inr err
+
+let rec get_fd_content (fd:file_descr) (t:IIO.Sig.trace) : option string =
+  match t with
+  | [] -> None
+  | (ERead fd' (Inl msg')) :: tl -> if fd = fd' then (Some msg') else (get_fd_content fd tl)
+  | (ERead fd' (Inr msg')) :: tl -> if fd = fd' then None else (get_fd_content fd tl)
+  | _ :: tl -> get_fd_content fd tl
+  
+let rec get_content (fnm:string) (t:IIO.Sig.trace) : option string =
+  match t with
+  | [] -> None
+  | (EOpenfile fnm' (Inl fd')) :: tl -> if fnm = fnm' then (get_fd_content fd' tl) else (get_content fnm tl)
+  | (EOpenfile fnm' (Inr fd')) :: tl -> if fnm = fnm' then None else (get_content fnm tl)
+  | _ :: tl -> get_content fnm tl
+
+val tp1 : trace_property #event
+let tp1 (tr:trace) =
+  match tr with
+  | Infinite_trace _ -> False
+  | Finite_trace t r -> 
+    match get_content "config.txt" t with
+    | Some msg1 -> strlen msg1 == r
+    | None -> r == 0
+
+(** Non-interference of secret **)
+val hyperprop_tp1 : unit ->  Lemma (
+  forall (tr1 tr2:trace). tr1 `member_of` tp1 /\ tr2 `member_of` tp1 ==> 
+  (match tr1, tr2 with
+  | Finite_trace t1 r1, Finite_trace t2 r2 -> (
+    get_content "config.txt" t1 == get_content "config.txt" t2 ==> r1 == r2)))
+let hyperprop_tp1 () = ()
+
+let whole1 () : IIO int AllActions 
+  (requires (fun _ -> True))
+  (ensures (fun _ r lt -> tp1 (Finite_trace lt r))) =
+  let config = read_content "config.txt" in
+  let secret = read_content "secret.txt" in
+  match config with
+  | Inl msg -> strlen msg
+  | Inr err -> 0
+
+(** Non-interference of secret **)
+val hyperprop_whole1 : unit -> Lemma (
+  forall (tr1 tr2:trace). tr1 `member_of` (beh whole1) /\ tr2 `member_of` (beh whole1) ==>
+  (match tr1, tr2 with
+  | Finite_trace t1 r1, Finite_trace t2 r2 -> (
+    get_content "config.txt" t1 == get_content "config.txt" t2 ==> r1 == r2)
+  | _, _ -> False))
+let hyperprop_whole1 () = 
+  assume (beh whole1 `subset_of` tp1);
+  assert (forall (tr:trace). tr `member_of` (beh whole1) ==> tr `member_of` tp1);
+  hyperprop_tp1 ();
+  ()
